% \lesson{1}{di 01 okt 2019 10:33}{Introduction}


% \begin{itemize}
%     \item First part: fundamental groups. We follow Munkres:
%         \begin{itemize}
%             \item Chap 9 `Fundamental group'
%             \item Chap 11 `The Seifert-Van Kampen thm' and
%             \item Chap 12/13 `Classification covering spaces'
%         \end{itemize}
%     \item Second part: Homology groups, via cudi, chapter of a book.
%     \item 10 problems (solve them during the semester) No feedback during the semester, but asking questions is allowed. Working together is allowed.
%     \item Exam (completely open book) First 4 questions: 1h30 prep. Last one 30 min, no prep
%         \begin{enumerate}
%             \item Theoretical question (open book, explain the proof, \ldots) \hfill /4
%             \item New problem (comparable to one of the 10 problems)\hfill /4
%             \item Explain your solution $n$-th problem solved at home \hfill /4
%             \item Explain your solution $m$-th problem solved at home\hfill /4
%             \item 4 small questions \hfill /4
%         \end{enumerate}
%         After the exam, hand in your solutions of the other problems. After a quick look, the points of 3.\ and 4.\ can be $\pm 1$ (in extreme cases $\pm 2$)
%     \item No exercise classes for this course!
% \end{itemize}

\setcounter{chapter}{0}
\chapter{Rings and Ideals}

\section{Rings and Ring homomorphisms}

\begin{definition}[Ring]
    A \term{ring} \( A \) is a set with two binary operations (addition and multiplication) such that:
    \begin{enumerate}
        \item \( A \) is an abelian group with respect to addition (so that \( A \) has a zero element, denoted by \( 0 \), and every \( x \in A \) has an additive inverse \( -x \)).
        \item Multiplication is associative and distributive over addition:
        \[
        (xy)z = x(yz), \quad x(y + z) = xy + xz, \quad (y + z)x = yx + zx.
        \]
        \item \( xy = yx \) for all \( x, y \in A \) (commutativity).
        \item There exists \( 1 \in A \) such that \( x1 = 1x = x \) for all \( x \in A \) (identity element).
    \end{enumerate}
\end{definition}
    
\begin{remark}
If \( 1 = 0 \), then for any \( x \in A \), we have
\[
x = x1 = x0 = 0,
\]
and so \( A \) has only one element, \( 0 \). In this case, \( A \) is the \term{zero ring}, denoted by \( 0 \).
\end{remark}
    
\begin{definition}[Ring Homomorphism]
A \term{ring homomorphism} is a mapping \( f: A \to B \) between rings \( A \) and \( B \) such that:
\begin{enumerate}
    \item \( f(x + y) = f(x) + f(y) \),
    \item \( f(xy) = f(x)f(y) \),
    \item \( f(1) = 1 \).
\end{enumerate}
\end{definition}

\begin{definition}[Subring] A subset \( S \subseteq A \) is a
\term{subring} if it is closed under addition and multiplication and
contains the identity element of \( A \). \end{definition}
    
% Functor from category of topological spaces to the category of groups.
% \begin{itemize}
%     \item Category: set of spaces and morphisms.
%     \item Functor: $X \leadsto G_X$ and  $f:X\to Y \leadsto f_*: G_X \to  G_Y$ such that
%         \begin{itemize}
%             \item $(f \circ g)_* = f_* \circ g_* $
%             \item $(1_X)_* = 1_{G_X}$
%         \end{itemize}
% \end{itemize}

% Two systems we'll discuss:
% \begin{itemize}
%     \item fundamental groups
%     \item homology groups
% \end{itemize}


% \begin{eg}
%     Suppose we have a functor.
%     If $G_X \not\cong G_Y$, then  $X$ and  $Y$ are not homeomorphic.
%     If `shadows' are different, then objects themselves are different too.
% \end{eg}
% \begin{explanation}
%     Suppose $X$ and $Y$ are homeomorphic.
%     Then $\exists f: X \to  Y$ and $g: Y \to  X$, maps (maps are always continuous in this course), such that $g  \circ f = 1_X$ and $f \circ g = 1_Y$.
%     Then $f_*: G_X \to G_Y$ and $g_*: G_Y \to  G_X$ such that $(g \circ f)_* = (1_X)_*$ and  $(f \circ g)_* = (1_Y)_*$. Using the rules discussed previously, we get
%     \[
%     g_*  \circ f_* = 1_{G_X} \quad f_*  \circ  g_* = 1_{G_Y}
%     ,\] 
%     which means that $f_* : G_X \to  G_Y$ is an isomorphism.
% \end{explanation}

\section{Ideals. Quotient Rings}

\begin{definition}[Ideal]
    An \term{ideal} \( \mathfrak{a} \subseteq A \) is a subset which is an additive subgroup and satisfies \( A\mathfrak{a} \subseteq \mathfrak{a} \), i.e., for all \( x \in A \), \( y \in \mathfrak{a} \), we have \( xy \in \mathfrak{a} \).
    \end{definition}
    
    \begin{definition}[Quotient Ring]
    Given a ring \( A \) and an ideal \( \mathfrak{a} \subset A \), the \term{quotient ring} \( A/\mathfrak{a} \) is the additive quotient group equipped with multiplication induced from \( A \), where the elements are cosets of \( \mathfrak{a} \), and the mapping
    \[
    \varphi: A \to A/\mathfrak{a}, \quad x \mapsto x + \mathfrak{a}
    \]
    is a surjective ring homomorphism.
    \end{definition}
    
    \begin{theorem}[First Isomorphism Theorem]
        Given a ring homomorphism \( \varphi: A \to B \), we have an isomorphism
        \[
        \varphi(A) \cong A / \ker \varphi.
        \]
    \end{theorem}
    
    \begin{theorem}[Second Isomorphism Theorem]
        Given an ideal \( \mathfrak{a} \subseteq A \), there is a one-to-one, order-preserving correspondence between the ideals \( \mathfrak{b}' \supseteq \mathfrak{a} \) in \( A \) and the ideals \( \mathfrak{b} \) in \( A/\mathfrak{a} \), given by
        \[
        \begin{array}{c@{\quad}c@{\quad}c}
        A & \xrightarrow{\hspace{1.2cm}\pi\hspace{0.5cm}} & A/\mathfrak{a} \\
        \mathfrak{a} \subseteq \mathfrak{b}' & \xleftrightarrow{\hspace{1.2cm}} & \mathfrak{b}
        \end{array}
        \]
    \end{theorem}

\section{Prime ideals and Maximal Ideals}

\begin{theorem}
Every ring \( A \ne (0) \) has at least one maximal ideal.
\end{theorem}

\begin{corollary}
If \( \mathfrak{a} \ne (1) \) is an ideal of \( A \), there exists a maximal ideal of \( A \) containing \( \mathfrak{a} \).
\end{corollary}

\begin{corollary}
Every non-unit \( a \in A \) is contained in a maximal ideal.
\end{corollary}

\leavevmode\vspace{0.5em} % forces line break after "Remark."

\textbf{Remarks.}

\begin{enumerate}
    \item If \( A \) is Noetherian (Chapter 7), we can avoid the use of Zorn’s lemma: the set of all ideals \( \ne (1) \) has a maximal element.
    \item There exist rings with exactly one maximal ideal, for example: local rings. A ring \( A \) with exactly one maximal ideal is called a \term{local ring}. The field \( k = A / \mathfrak{m} \) is called the \term{residue field} of \( A \).
\end{enumerate}

% \begin{remark}
%     \leavevmode\vspace{0.5em} % forces line break after "Remark."
%     \begin{enumerate}
%     \item If \( A \) is Noetherian (Chapter 7), we can avoid the use of Zorn’s lemma: the set of all ideals \( \ne (1) \) has a maximal element.
%     \item There exist rings with exactly one maximal ideal, for example: local rings. A ring \( A \) with exactly one maximal ideal is called a \term{local ring}. The field \( k = A / \mathfrak{m} \) is called the \term{residue field} of \( A \).
% \end{enumerate}
% \end{remark}

\begin{prop}
    \begin{enumerate}[label=\textnormal{(\roman*)}]
        \item Let \( A \) be a ring and \( \mathfrak{m} \) an ideal of \( A \) such that every \( x \in A - \mathfrak{m} \) is a unit in \( A \). Then \( A \) is a local ring and \( \mathfrak{m} \) its maximal ideal.
        \item Let \( A \) be a ring and \( \mathfrak{m} \) a maximal ideal of \( A \), such that every element of \( 1 + \mathfrak{m} \) (i.e., every \( 1 + x \), where \( x \in \mathfrak{m} \)) is a unit in \( A \). Then \( A \) is a local ring.
    \end{enumerate}
\end{prop}
A ring with only a finite number of maximal ideals is called \term{semi-local}.

\begin{eg}
Let \( A = k[x_1, \ldots, x_n] \), where \( k \) is a field. Let \( f \in A \) be an irreducible polynomial. By unique factorization, the ideal \( (f) \) is prime.
\end{eg}

\begin{eg}
Let \( A = \mathbb{Z} \). Every ideal in \( \mathbb{Z} \) is of the form \( (m) \) for some \( m \ge 0 \). The ideal \( (m) \) is prime \( \Leftrightarrow m = 0 \) or a prime number. All the ideals \( (p) \), where \( p \) is a prime number, are maximal: \( \mathbb{Z}/(p) \) is the field of \( p \) elements.
\end{eg}

\begin{remark}
The same holds in Example 1 for \( n = 1 \), but not for \( n > 1 \). 
The ideal \( \mathfrak{m} \) of all polynomials in \( A = k[x_1, 
\ldots, x_n] \) with zero constant term is maximal (since it is the 
kernel of the homomorphism \( A \to k \), which maps \( f \in A \) to 
\( f(0) \)). But if \( n > 1 \), \( \mathfrak{m} \) is not a principal
 ideal (requires at least \( n \) generators).
\end{remark}

\begin{eg}
A \term{principal ideal domain} is an integral domain in which every ideal is principal. In such a ring, every non-zero prime ideal is maximal.

For if \( (x) \ne 0 \) is a prime ideal and \( (y) \supset (x) \), we have \( x \in (y) \), say \( x = yz \), so that \( yz \in (x) \) and \( y \notin (x) \), hence \( z \in (x) \); say \( z = tx \). Then \( x = ytx \), so that \( yt = 1 \), and therefore \( (y) = (1) \).
\end{eg}



        
        
% \section{Prime ideals & Maximal Ideals}

% \begin{theorem}[Second Isomorphism Theorem]
%         Given an ideal \( \mathfrak{a} \subseteq A \), there is a one-to-one, order-preserving correspondence between the ideals \( \mathfrak{b}' \supseteq \mathfrak{a} \) in \( A \) and the ideals \( \mathfrak{b} \) in \( A/\mathfrak{a} \), given by
%         \[
%         \begin{array}{c@{\quad}c@{\quad}c}
%         A & \xrightarrow{\hspace{1.2cm}\pi\hspace{0.5cm}} & A/\mathfrak{a} \\
%         \mathfrak{a} \subseteq \mathfrak{b}' & \xleftrightarrow{\hspace{1.2cm}} & \mathfrak{b}
%         \end{array}
%         \]
%     \end{theorem}
        
        
    

% Pick a base point $x_0$ and consider it fixed. (The fundamental group will not depend on it. We assume all spaces are path connected)
% $X \leadsto \pi(X)$.
% \begin{itemize}
%     \item A loop based at $x_0 \in X$ is a map $f: I = [0, 1] \to X$, $f(0) = f(1) = x_0$.
%     \item Loops are equivalent if one can be deformed in the other in a continuous way, with the base point fixed.
%     \item The fundamental group consists of equivalent classes of loops.
% \end{itemize}

% \begin{eg}
%     Let $X = B^2$ (2 dimensional disk).
%     Then $\pi(B^2) = 1$, because every loop is equivalent to the `constant' loop.
% \end{eg}
% \begin{eg}
%     Let $X = S^{1}$ and pick $x_0$ on the circle.
%     Two options: 
%     \begin{itemize}
%         \item The loop is trivial equivalent to the constant loop
%         \item The loop goes around the circle.
%         \item The loop goes around the circle, twice.
%         \item The loop goes around the circle, clockwise, once
%         \item \ldots
%     \end{itemize}
%     $\pi(S^{1}) \cong \Z$ (proof will follow).
% \end{eg}

% The composition of loops is simply pasting them.
% In the case of the circle, the loop $-1$  $\circ$ the loop  $2$ is the loop $1$.

% Suppose $\alpha: I \to  X$ and $f : X\to Y$. Then we define 
% \[
%     f_*[\alpha] = [f \circ \alpha]
% .\] 


% \begin{theorem}[Fixed point theorem of Brouwer]
%     Any continuous map from a rectangle to itself has at least one fixed point.
% \end{theorem}
% \begin{proof}
%     Suppose there is no fixed point, so $f(x) \neq x$ for all  $x \in B^2$.
%     Then we can construct map $r : B^2 \to  S_1$ as follows:
%     take the intersection of the boundary and half ray between $f(x)$ and $x$.
%     \begin{figure}[H]
%         \centering
%         \incfig{proof-fixed-point-brouwer}
%         \caption{Proof of the Brouwer fixed point theorem}
%         \label{fig:proof-fixed-point-brouwer}
%     \end{figure}
%     If $x$ lies on the boundary, we have the identity map.
%     This map is continuous.
%     Then we have $S^1 \to B^2 \to S^1$, via the inclusion and $r$.
%     Looking at the fundamental groups:
%     \[
%         \pi(S^1)  =\Z \to  \pi(B^2) = 1 \to  \pi(S^1) = \Z
%     .\] 
%     The map from $\pi(S^1) \to  \pi(S^{1})$ is the identity map, but the first map maps everything on $1$. \phantom\qedhere\hfill\contra 
% \end{proof}



% \setcounter{chapter}{1}
% \chapter{Fundamental group}

% \setcounter{section}{50}
% \section{Homotopy of paths}
% \begin{definition}[Homotopy]
%     Let $f,g:X\to Y$ be maps (so continuous). Then a homotopy between $f$ and $g$ is a continuous map $H: X\times I \to Y$ such that
%     \begin{itemize}
%         \item $H(x, 0) = f(x)$, $H(x, 1) = g(x)$ 
%         \item For all $t \in I$, define $f_t: X \to  Y: x \mapsto  H(x, t)$
%     \end{itemize}
%     We say that $f$ is homotopic with $g$, we write $f \simeq g$.
%     If $g$ is a constant map, we say that $f$ is null homotopic.
% \end{definition}

% \begin{definition}[Path homotopy]
%     Let $f, g: I \to  X$ be two paths such that $f(0) = g(0) = x_0$ and $f(1) = g(1) = x_1$. Then $H: I \times  I \to  X$ is a path homotopy between $f$ and $g$, if and only if
%     \begin{itemize}
%         \item $H(s,0) = f(s)$ and  $H(s, 1) = g(s)$ (homotopy between maps)
%         \item  $H(0, t) = x_0$ and $H(1, t) = x_1$ (start and end points fixed)
%     \end{itemize}
%     Notation: $f \simeq_p g$.
% \end{definition}


% \begin{figure}[ht]
%     \centering
%     \incfig{homotopy-general-example}
%     \caption{General example of a homotopy.}
%     \label{fig:homotopy-general-example}
% \end{figure}


% \begin{lemma}
%     $\simeq$ and  $\simeq_p$ are equivalence relations.
% \end{lemma}
% \begin{proof}
%     \leavevmode
%     \begin{itemize}
%         \item Reflective: $F(x, t) = f(x)$
%         \item Symmetric: $G(x, t) = H(x, 1-t)$ 
%         \item Transitive:  Suppose $f \simeq g$ and  $g \simeq h$, with  $H_1, H_2$ resp.
%             \[
%                 H(x, t) = \begin{cases}
%                     H_1(x, 2t) & 0 \le t \le  \frac{1}{2}\\
%                     H_2(x, 2t-1) & \frac{1}{2} \le  t \le  1
%                 \end{cases}
%             . \qedhere
%         \] 
%     \end{itemize}
% \end{proof}


% \begin{eg}[Trivial, but important]
%    Let $C \subset \R^n$ be a convex subset.
%    \begin{itemize}
%        \item Any two maps $f, g: X \to C$ are homotopic.
%        \item Any two paths $f, g: I \to  C$ with $f(0) = g(0)$ and  $g(1) = f(1)$ are path homotopic.
%    \end{itemize}

%    Choose $H: X \times I \to  C: (x, t) \to  H(x, t) = (1-t) f(x) + t g(x)$.
% \end{eg}


% \subsection*{Product of paths}
% Let $f: I\to X$, $g: I \to X$ be paths, $f(1) = g(0)$.
% Define  \[
%     f*g: I \to X: s \mapsto \begin{cases}
%         f(2s) & 0 \le  s \le  \frac{1}{2}\\
%         g(2s - 1) & \frac{1}{2}\le s\le 1.
% \end{cases}
% \]
% \begin{remark}
%     If $f$ is path homotopic to $f'$ and $g$ path homotopic to $g'$ (which means that $f(1) = f'(1) = g(0) = g'(0)$), then $f * g \simeq_p f' * g'$.
% \end{remark}

% So we can define $[f] * [g] := [f*g]$ with $[f] := \{g : I \to  X  \mid g \simeq_p f\} $

% \begin{theorem}\leavevmode
%     \begin{enumerate}
%         \item $[f] * ([g] * [h])$  is defined iff $([f] * [g])*[h]$ is defined and in that case, they are equal.
%         \item Let $e_x$ denote the constant path $e_x: I \to  X: s \mapsto x$, $x \in X$. If $f(0) = x_0$ and $f(1) = x_1$ then $[e_{x_0}] * [f] = [f]$ and $[f] * [e_{x_1}] = [f]$.
%         \item Let $\overline{f} : I \to  X: s \mapsto  f(1-s)$. Then $[f] * [\overline{f}] = [e_{x_0}]$ and $[\overline{f}]*[f] = [e_{x_1}]$
%     \end{enumerate}
% \end{theorem}
% \begin{proof}
%     First, two observations
%     \begin{itemize}
%         \item Suppose $f\simeq_p g$ via homotopy $H$, $f, g: I\to X$.
%             Let $k: X \to  Y$.
%             Then $k  \circ  f \simeq_p k \circ g$ using $k  \circ H$.
%         \item If $f*g$ (not necessarily path homotopic). Then $ k  \circ (f*g) = (k \circ f) * (k \circ g) .$ 
%     \end{itemize}

%     Now, the proof
%     \begin{itemize}
%         \item[2.]  Take $e_0: I \to  I: s \mapsto 0$.
%             Take $i: I \to  I: s \mapsto s$ 
%             Then $e_0*i$ is a path from $0$ to $1 \in I$.
%             The path $i$ is also such a path.
%             Because $I$ is a convex subset, $e_0*i$ and $i$ are path homotopic, $e_0 *i\simeq_p i$.
%             Using one of our observations, we find that
%             \begin{align*}
%                 f  \circ (e_0 * i) &\simeq_p  f  \circ i\\
%                 (f  \circ  e_0) * (f  \circ  i ) &\simeq_p f\\
%                 e_{x_0} * f  &\simeq_p f\\
%                 [e_{x_0}] * [f]  &= [f]
%             .\end{align*}

%         \item [3.] Note that $i * \overline{i} \simeq_p e_0$.
%             Now, applying the same rules, we get 
%             \begin{align*}
%                 f  \circ (i * \overline{i}) &\simeq_p f  \circ  e_0\\
%                 f * \overline{f} &\simeq_p  e_{x_0}\\
%                 [f] * [\overline{f}] & = [e_{x_0}]
%             .\end{align*}
%         \item[1.]  Remark: Only defined if $f(1) = g(0), g(1) = h(0)$.
%             Note that $f*(g*h) \neq (f*g)*h$. The trajectory is the same, but the speed is not.

%             Assume the product is defined.
%             Suppose $[a, b]$,  $[c, d]$ are intervals in  $\R$.
%             Then there is a unique positive (positive slope), linear map from $[a, b] \to [c,d]$.
%             For any $a, b \in [0, 1)$ with $ 0<a<b<1$, we define a path
%             \begin{align*}
%                 k_{a,b}: [0, 1] &\longrightarrow  X\\
%                 [0, a] & \xrightarrow{\text{lin.}}[0, 1] \xrightarrow{f}  X\\
%                 [a, b] & \xrightarrow{\text{lin.}}[0, 1] \xrightarrow{g}  X\\
%                 [b, 0] & \xrightarrow{\text{lin.}}[0, 1] \xrightarrow{h}  X\\
%             \end{align*} 

%             Then $f*(g*h) = k_{\frac{1}{2}, \frac{3}{4}}$ and $(f*g)*h = k_{\frac{1}{4}, \frac{1}{2}}$

%             Let $\gamma$ be that path $\gamma:I \to  I$ with the following graphs:

%             \begin{figure}[H]
%                 \centering
%                 \incfig{proof-path}
%                 \caption{proof path}
%                 \label{fig:proof-path}
%             \end{figure}
%             Note  that $\gamma \simeq_p i$.
%             Now, using the fact that composition of positive linear maps is positive linear.
%             \begin{align*}
%                 k_{c, d}  \circ  \gamma &\simeq_p  k_{c, d}  \circ i\\
%                 k_{a, b} &\simeq_p  k_{c, d},
%             \end{align*} 
%             which is what we wanted to show.
%     \end{itemize}
% \end{proof}


% \section{Fundamental group}
% \begin{definition}
%     Let $X$ be a space and $x_0 \in X$, then the fundamental group of $X$ based at $x_0$ is
%     \[
%         \pi(X, x_0) = \{ [f]  \mid  f : I \to X, f(0) = f(1) = x_0\} 
%     .\] 
%     (Also $\pi_1(X, x_0)$ is used, first homotopy group of $X$ based at $x_0$)

%     For $[f], [g] \in \pi(X, x_0)$, $[f] * [g]$ is always defined,  $[e_{x_0}]$ is an identity element, $*$ is associative and $[f]^{-1} = [\overline{f}]$. This makes $(\pi(X, x_0), *)$ a group.
% \end{definition}
% \begin{eg}
%     If $C \subset \R^n$, convex then $\pi(X, x_0) = 1$.
%     E.g. $\pi(B^2, x_0) = 1$.
% \end{eg}

% \begin{remark}
%     All groups are a fundamental group of some space.
% \end{remark}

% Question: how does the group depend on  the base point?

% \begin{theorem}[52.1]
%     Let $X$ be a space, $x_0, x_1 \in X$ and $\alpha: I \to X$ a path from  $x_0$ to $x_1$.
%     Then
%     \begin{align*}
%         \hat{\alpha}: \pi(X, x_0) &\longrightarrow\pi(x, x_1)\\
%         [f] &\longmapsto  [\overline{\alpha}] * [f] * [\alpha]
%     .\end{align*}
%     is an isomorphisms of groups. Note however that this isomorphism depends on $\alpha$.
% \end{theorem}
% \begin{proof}
%     Let $[f], [g] \in \pi_1(X, x_0)$.
%     Then 
%     \begin{align*}
%         \hat{\alpha}([f]*[g]) &= [\overline{\alpha}] * [f] * [g] * [\alpha]\\
%                               &= [\overline{\alpha}] *[f] * [\alpha] * [\overline{\alpha}] * [g] * [\alpha]\\
%                               &= \hat{\alpha}[f] * \hat{\alpha}[g]
%     .\end{align*}
%     We can also construct the inverse, proving that these groups are isomorphic.
% \end{proof}

% \begin{figure}[ht]
%     \centering
%     \incfig{dependence-of-base-point}
%     \caption{Construction of the group homomorphism}
%     \label{fig:dependence-of-base-point}
% \end{figure}
% \begin{remark}
%     If $f: (x, x_0) \to (Y, y_0)$ is a map of pointed topology spaces ($f: X \to Y$ continuous and $f(x_0) = y_0$).
%     Then \[
%         f_*:\pi(X, x_0) \to  \pi(Y, y_0): [\gamma] \mapsto [f  \circ \gamma]
%     \]
%     is a morphism of groups, because of the two `rules' discussed previously, with
%     \[
%         (f \circ g)_* = f_*  \circ g_* \qquad (1_X)_* = 1_{\pi(X, x_0)}
%     .\] 
% \end{remark}
